replace refcounts with successor-list in BlockCache

disk-betree/BlockCacheSystem.dfy
@@ -73,13 +73,8 @@ abstract module BlockCacheSystem {
   requires WFSuperblockWrtDisk(k, DiskSuperblock(k, s.disk.blocks), s.disk.blocks)
   {
     Graph(
-      DiskSuperblock(k, s.disk.blocks).refcounts.Keys,
+      DiskSuperblock(k, s.disk.blocks).graph.Keys,
       RefMapOfDisk(k, DiskSuperblock(k, s.disk.blocks), s.disk.blocks))
-  }
-
-  function {:opaque} Predecessors(graph: map<Reference, Node>, ref: Reference) : set<Reference>
-  {
-    set r | r in graph && ref in M.G.Successors(graph[r])
   }
 
   predicate NoDanglingPointers(graph: map<Reference, Node>)
@@ -89,9 +84,10 @@ abstract module BlockCacheSystem {
       :: r2 in graph
   }
 
-  predicate RefcountsAgree(refcounts: map<Reference, int>, graph: map<Reference, Node>)
+  predicate SuccessorsAgree(succGraph: map<Reference, seq<Reference>>, graph: map<Reference, Node>)
   {
-    forall ref | ref in refcounts :: refcounts[ref] == |Predecessors(graph, ref)|
+    && succGraph.Keys == graph.Keys
+    && forall ref | ref in succGraph :: (iset r | r in succGraph[ref]) == M.G.Successors(graph[ref])
   }
 
   predicate Init(k: Constants, s: Variables)
@@ -100,7 +96,7 @@ abstract module BlockCacheSystem {
     && D.Init(k.disk, s.disk)
     && WFDisk(k, s.disk.blocks)
     && WFSuperblockWrtDisk(k, DiskSuperblock(k, s.disk.blocks), s.disk.blocks)
-    && RefcountsAgree(DiskSuperblock(k, s.disk.blocks).refcounts, PersistentGraph(k, s))
+    && SuccessorsAgree(DiskSuperblock(k, s.disk.blocks).graph, PersistentGraph(k, s))
     && NoDanglingPointers(PersistentGraph(k, s))
   }
 
@@ -140,11 +136,8 @@ abstract module BlockCacheSystem {
   requires WFDisk(k, s.disk.blocks)
   requires WFSuperblockWrtDisk(k, s.machine.ephemeralSuperblock, s.disk.blocks)
   {
-    /*assert s.machine.ephemeralSuperblock.refcounts.Keys
-        <= s.machine.ephemeralSuperblock.lbas.Keys + s.machine.cache.Keys
-        == MapUnionPreferB(RefMapOfDisk(k, s.machine.ephemeralSuperblock, s.disk.blocks), s.machine.cache.Keys;*/
     Graph(
-      s.machine.ephemeralSuperblock.refcounts.Keys,
+      s.machine.ephemeralSuperblock.graph.Keys,
       MapUnionPreferB(RefMapOfDisk(k, s.machine.ephemeralSuperblock, s.disk.blocks), s.machine.cache)
     )
   }
@@ -164,12 +157,12 @@ abstract module BlockCacheSystem {
     && M.Inv(k.machine, s.machine)
     && WFDisk(k, s.disk.blocks)
     && WFSuperblockWrtDisk(k, DiskSuperblock(k, s.disk.blocks), s.disk.blocks)
-    && RefcountsAgree(DiskSuperblock(k, s.disk.blocks).refcounts, PersistentGraph(k, s))
+    && SuccessorsAgree(DiskSuperblock(k, s.disk.blocks).graph, PersistentGraph(k, s))
     && NoDanglingPointers(PersistentGraph(k, s))
     && (s.machine.Ready? ==>
       && s.machine.persistentSuperblock == DiskSuperblock(k, s.disk.blocks)
       && WFSuperblockWrtDisk(k, s.machine.ephemeralSuperblock, s.disk.blocks)
-      && RefcountsAgree(s.machine.ephemeralSuperblock.refcounts, EphemeralGraph(k, s))
+      && SuccessorsAgree(s.machine.ephemeralSuperblock.graph, EphemeralGraph(k, s))
       && NoDanglingPointers(EphemeralGraph(k, s))
       && CleanCacheEntriesAreCorrect(k, s)
     )
@@ -225,12 +218,6 @@ abstract module BlockCacheSystem {
         == RefMapOfDisk(k, s.machine.ephemeralSuperblock, s.disk.blocks)
         == MapUnionPreferB(RefMapOfDisk(k, s.machine.ephemeralSuperblock, s.disk.blocks), s.machine.cache);
     assert PersistentGraph(k, s') == EphemeralGraph(k, s);
-
-    //assert RefcountsAgree(DiskSuperblock(k, s'.disk.blocks).refcounts, PersistentGraph(k, s'));
-
-    //assert s'.machine.persistentSuperblock == DiskSuperblock(k, s'.disk.blocks);
-    //assert WFSuperblockWrtDisk(k, s'.machine.ephemeralSuperblock, s'.disk.blocks);
-    //assert RefcountsAgree(s'.machine.ephemeralSuperblock.refcounts, EphemeralGraph(k, s'));
   }
 
   lemma WriteBackSuperblockStepPreservesInvariant(k: Constants, s: Variables, s': Variables, dop: DiskOp)
@@ -242,164 +229,18 @@ abstract module BlockCacheSystem {
     WriteBackSuperblockStepSyncsGraphs(k, s, s', dop);
   }
 
-  lemma PredecessorsRemoveRef(k: Constants, s: Variables, graph: map<Reference, Node>, r: Reference, ref: Reference)
-  requires M.Inv(k.machine, s.machine)
-  requires WFDisk(k, s.disk.blocks)
-  requires s.machine.Ready?
-  requires WFSuperblockWrtDisk(k, s.machine.ephemeralSuperblock, s.disk.blocks)
-  requires graph == EphemeralGraph(k, s)
-  requires ref in s.machine.ephemeralSuperblock.lbas ==> ref in s.machine.cache
-  ensures |Predecessors(graph, r)|
-      - (if ref in s.machine.cache && r in M.G.Successors(s.machine.cache[ref]) then 1 else 0)
-      == |Predecessors(graph, r) - {ref}|;
-  {
-    reveal_Predecessors();
-  }
-
-  lemma PredecessorsGraphMinusRefInclusion(
-    k: Constants,
-    s: Variables,
-    s': Variables,
-    graph: map<Reference, Node>,
-    graph': map<Reference, Node>,
-    r: Reference,
-    ref: Reference)
-  requires M.Inv(k.machine, s.machine)
-  requires M.Inv(k.machine, s'.machine)
-  requires WFDisk(k, s.disk.blocks)
-  requires s.disk == s'.disk
-  requires s.machine.Ready?
-  requires s'.machine.Ready?
-  requires WFSuperblockWrtDisk(k, s.machine.ephemeralSuperblock, s.disk.blocks)
-  requires WFSuperblockWrtDisk(k, s'.machine.ephemeralSuperblock, s'.disk.blocks)
-  requires graph == EphemeralGraph(k, s)
-  requires graph' == EphemeralGraph(k, s')
-  requires ref in s.machine.ephemeralSuperblock.lbas ==> ref in s.machine.cache
-  requires ref in s'.machine.ephemeralSuperblock.lbas ==> ref in s'.machine.cache
-  requires MapRemove(s.machine.cache, {ref}) == MapRemove(s'.machine.cache, {ref})
-  requires MapRemove(s.machine.ephemeralSuperblock.lbas, {ref}) == MapRemove(s'.machine.ephemeralSuperblock.lbas, {ref})
-  ensures forall r1 | r1 in Predecessors(graph, r) - {ref} ::
-      r1 in Predecessors(graph', r) - {ref}
-  {
-    forall r1 | r1 in Predecessors(graph, r) - {ref}
-    ensures r1 in Predecessors(graph', r) - {ref}
-    {
-      assert r1 != ref;
-      if (r1 in s'.machine.ephemeralSuperblock.lbas) {
-        assert r1 in MapRemove(s'.machine.ephemeralSuperblock.lbas, {ref});
-        assert r1 in MapRemove(s.machine.ephemeralSuperblock.lbas, {ref});
-        assert r1 in s.machine.ephemeralSuperblock.lbas;
-        assert s.machine.ephemeralSuperblock.lbas[r1] == 
-               s'.machine.ephemeralSuperblock.lbas[r1];
-        assert RefMapOfDisk(k, s.machine.ephemeralSuperblock, s.disk.blocks)[r1]
-            == RefMapOfDisk(k, s'.machine.ephemeralSuperblock, s'.disk.blocks)[r1];
-      }
-      if (r1 in s.machine.ephemeralSuperblock.lbas) {
-        assert r1 in MapRemove(s.machine.ephemeralSuperblock.lbas, {ref});
-        assert r1 in MapRemove(s'.machine.ephemeralSuperblock.lbas, {ref});
-        assert r1 in s'.machine.ephemeralSuperblock.lbas;
-        assert s'.machine.ephemeralSuperblock.lbas[r1] == 
-               s.machine.ephemeralSuperblock.lbas[r1];
-        assert RefMapOfDisk(k, s.machine.ephemeralSuperblock, s.disk.blocks)[r1]
-            == RefMapOfDisk(k, s'.machine.ephemeralSuperblock, s'.disk.blocks)[r1];
-      }
-
-      reveal_Predecessors();
-
-      if (r1 in s.machine.cache) {
-        assert s.machine.cache.Keys - {ref} == s'.machine.cache.Keys - {ref};
-        assert r1 in (s.machine.cache.Keys - {ref});
-        assert r1 in (s'.machine.cache.Keys - {ref});
-        assert r1 in s'.machine.cache;
-        assert graph[r1] == s.machine.cache[r1]
-            == s'.machine.cache[r1]
-            == graph'[r1];
-        assert MapsTo(graph', r1, graph[r1]);
-      } else {
-        assert r1 in RefMapOfDisk(k, s'.machine.ephemeralSuperblock, s'.disk.blocks);
-        assert r1 in RefMapOfDisk(k, s.machine.ephemeralSuperblock, s.disk.blocks);
-        assert r1 in graph;
-        assert r1 in graph';
-        assert graph[r1]
-            == RefMapOfDisk(k, s.machine.ephemeralSuperblock, s.disk.blocks)[r1]
-            == RefMapOfDisk(k, s'.machine.ephemeralSuperblock, s'.disk.blocks)[r1]
-            == graph'[r1];
-        assert MapsTo(graph', r1, graph[r1]);
-      }
-      assert r1 in Predecessors(graph', r) - {ref};
-    }   
-  }
-
-  lemma RefcountConservation(k: Constants, s: Variables, s': Variables, graph: map<Reference, Node>, graph': map<Reference, Node>, ref: Reference, r: Reference)
-  requires Inv(k, s);
-  requires M.Inv(k.machine, s'.machine)
-  requires s'.machine.Ready?
-  requires s'.disk == s.disk
-  requires WFDisk(k, s'.disk.blocks)
-  requires WFSuperblockWrtDisk(k, s'.machine.ephemeralSuperblock, s'.disk.blocks)
-  requires s.machine.Ready?
-  requires s'.machine.Ready?
-  requires graph == EphemeralGraph(k, s)
-  requires graph' == EphemeralGraph(k, s')
-  requires ref in s.machine.ephemeralSuperblock.lbas ==> ref in s.machine.cache
-  requires ref in s'.machine.ephemeralSuperblock.lbas ==> ref in s'.machine.cache
-  requires MapRemove(s.machine.cache, {ref}) == MapRemove(s'.machine.cache, {ref})
-  requires MapRemove(s.machine.ephemeralSuperblock.lbas, {ref}) == MapRemove(s'.machine.ephemeralSuperblock.lbas, {ref})
-
-  ensures |Predecessors(graph, r)| - (if ref in s.machine.cache && r in M.G.Successors(s.machine.cache[ref]) then 1 else 0)
-       == |Predecessors(graph', r)| - (if ref in s'.machine.cache && r in M.G.Successors(s'.machine.cache[ref]) then 1 else 0)
-  {
-    PredecessorsRemoveRef(k, s, graph, r, ref);
-    PredecessorsRemoveRef(k, s', graph', r, ref);
-
-    PredecessorsGraphMinusRefInclusion(k, s, s', graph, graph', r, ref);
-    PredecessorsGraphMinusRefInclusion(k, s', s, graph', graph, r, ref);
-    assert Predecessors(graph, r) - {ref} == Predecessors(graph', r) - {ref};
-  }
-
   lemma DirtyStepPreservesInvariant(k: Constants, s: Variables, s': Variables, ref: Reference, block: Node)
     requires Inv(k, s)
     requires M.Dirty(k.machine, s.machine, s'.machine, ref, block)
     requires s.disk == s'.disk
     ensures Inv(k, s')
   {
-    var refcounts := s.machine.ephemeralSuperblock.refcounts;
-    var refcounts' := s'.machine.ephemeralSuperblock.refcounts;
+    /*
     var graph := EphemeralGraph(k, s);
     var graph' := EphemeralGraph(k, s');
     var cache := s.machine.cache;
     var cache' := s'.machine.cache;
-
-    forall r | r in refcounts'
-    ensures refcounts'[r] == |Predecessors(graph', r)|
-    {
-      RefcountConservation(k, s, s', graph, graph', ref, r);
-
-      M.reveal_refCountsChangeConsistently();
-
-      /*
-      assert refcounts'[r]
-          == refcounts[r] +
-            (if ref in cache' && r in M.G.Successors(cache'[ref]) then 1 else 0) -
-            (if ref in cache && r in M.G.Successors(cache[ref]) then 1 else 0)
-          == |Predecessors(graph, r)| +
-            (if ref in cache' && r in M.G.Successors(cache'[ref]) then 1 else 0) -
-            (if ref in cache && r in M.G.Successors(cache[ref]) then 1 else 0)
-          == |Predecessors(graph', r)|;
-      */
-    }
-
-    forall r1, r2 | r1 in graph' && r2 in M.G.Successors(graph'[r1])
-    ensures r2 in graph'
-    {
-      if (r1 == ref) {
-        assert r2 in graph';
-      } else {
-        //assert graph[r1] == graph'[r1];
-        assert r2 in M.G.Successors(graph[r1]);
-        assert r2 in graph';
-      }
-    }
+    */
   }
 
   lemma AllocStepPreservesInvariant(k: Constants, s: Variables, s': Variables, ref: Reference, block: Node)
@@ -408,49 +249,12 @@ abstract module BlockCacheSystem {
     requires s.disk == s'.disk
     ensures Inv(k, s')
   {
-    var refcounts := s.machine.ephemeralSuperblock.refcounts;
-    var refcounts' := s'.machine.ephemeralSuperblock.refcounts;
+  /*
     var graph := EphemeralGraph(k, s);
     var graph' := EphemeralGraph(k, s');
     var cache := s.machine.cache;
     var cache' := s'.machine.cache;
-
-    forall r | r in refcounts'
-    ensures refcounts'[r] == |Predecessors(graph', r)|
-    {
-      M.reveal_refCountsChangeConsistently();
-      if (r == ref) {
-        //assert ref !in M.Successors(block);
-        //assert ref !in s.machine.cache;
-        //assert ref !in M.Successors(s'.machine.cache[ref]);
-
-        RefcountConservation(k, s, s', graph, graph', ref, r);
-        /*if (|Predecessors(graph, r)| != 0) {
-          var x :| x in Predecessors(graph, r);
-          assert r in M.Successors(graph[x]);
-          assert r in graph;
-          assert false;
-        }*/
-        reveal_Predecessors();
-        assert |Predecessors(graph, r)| == 0;
-
-        assert |Predecessors(graph', r)| == 0;
-        assert refcounts'[r] == 0;
-      } else {
-        RefcountConservation(k, s, s', graph, graph', ref, r);
-      }
-    }
-
-    forall r1, r2 | r1 in graph' && r2 in M.G.Successors(graph'[r1])
-    ensures r2 in graph'
-    {
-      if (r1 == ref) {
-        assert r2 in graph';
-      } else {
-        assert r2 in M.G.Successors(graph[r1]);
-        assert r2 in graph';
-      }
-    }
+    */
   }
 
   lemma OpPreservesInvariant(k: Constants, s: Variables, s': Variables, op: Op)
@@ -496,33 +300,12 @@ abstract module BlockCacheSystem {
     requires D.Stutter(k.disk, s.disk, s'.disk, dop);
     ensures Inv(k, s')
   {
-    var refcounts := s.machine.ephemeralSuperblock.refcounts;
-    var refcounts' := s'.machine.ephemeralSuperblock.refcounts;
+    /*
     var graph := EphemeralGraph(k, s);
     var graph' := EphemeralGraph(k, s');
     var cache := s.machine.cache;
     var cache' := s'.machine.cache;
-
-    forall r | r in refcounts'
-    ensures refcounts'[r] == |Predecessors(graph', r)|
-    {
-      assert r != ref;
-      RefcountConservation(k, s, s', graph, graph', ref, r);
-      M.reveal_refCountsChangeConsistently();
-      reveal_Predecessors();
-    }
-
-    forall r1, r2 | r1 in graph' && r2 in M.G.Successors(graph'[r1])
-    ensures r2 in graph'
-    {
-      if (r2 == ref) {
-        reveal_Predecessors();
-        assert false;
-      } else {
-        assert r2 in M.G.Successors(graph[r1]);
-        assert r2 in graph';
-      }
-    }
+    */
   }
 
   lemma PageInStepPreservesGraphs(k: Constants, s: Variables, s': Variables, dop: DiskOp, ref: Reference)
